Classes/Monad.v
@@ -7,11 +7,12 @@ Implicit Type M : Type → Type.
 Implicit Type T : (Type → Type) → Type → Type.
 Implicit Type A B C D : Type.
 
-Class Monad M `{Applicative M} : Type :=
+Class Monad M : Type :=
 {
+  is_applicative :> Applicative M;
   bindM : ∀ {A B}, M A  → (A → M B) → M B;
   bind_id_left : ∀ {A B} (f : A → M B) (a : A), 
-    bindM (pure a) f = f a;
+    bindM (@pure M is_applicative A a) f = f a;
   bind_id_right : ∀ {A} (MA : M A),
     bindM MA pure = MA;
   bind_assoc : ∀ {A B C} (MA : M A) (f : A → M B) (g : B → M C),
@@ -22,6 +23,7 @@ Class Monad M `{Applicative M} : Type :=
     bindM (f <$> x) g = bindM x (f ∘ g);
   bind_pass : ∀ {A B} (ma : M A) (mb : M B), ma >> mb = bindM ma (λ _, mb);
 }.
+
 Hint Rewrite @bind_id_left @bind_id_right @bind_assoc @bind_app : soundness.
 
 Definition composeM {M : Type → Type} `{Monad M}
@@ -40,7 +42,7 @@ Notation "x >=> y" := (composeM x y) (at level 40, left associativity).
 
 Section laws_and_methods.
   Context {M} `{Monad M}.
-  
+
   Definition join {A} (x : M (M A)) : M A := bindM x id.
 
   Lemma join_fmap {A : Type} (x : M(M(M(A)))) : 
