Instances/Monad.v
@@ -7,72 +7,84 @@ Require Import FunctionalExtensionality.
 Require Import Language.Statements.
 Require Import Types.Maps.
 
-Inductive Maybe (A : Type) : Type :=
+Implicit Type S A B C : Type.
+Implicit Type M : Type → Type.
+
+Inductive Maybe A : Type :=
     | Just : A -> Maybe A
     | None : Maybe A.
 Arguments Just {_}.
 Arguments None {_}.
 
 Section Maybe_Functor.
-  Definition fmap_maybe {A B : Type} (f : A -> B) (ma : Maybe A) : Maybe B :=
+  Definition fmap_maybe {A B} (f : A → B) ma : Maybe B :=
     match ma with
     | Just a => Just (f a)
     | None => None
     end.
-  Arguments fmap_maybe [_ _] _ _.
+  Arguments fmap_maybe [A B] f ma.
   Hint Unfold fmap_maybe : soundness.
 
-  Lemma fmap_maybe_id : ∀ A : Type, fmap_maybe (@id A) = id.
-  Proof. simple_solve. Qed.
+  Lemma fmap_maybe_id A : (fmap_maybe (B:=A)) id = id.
+  Proof. 
+    unfold fmap_maybe. ext. destruct x; reflexivity.
+  Qed.
+  Arguments fmap_maybe_id [A].
 
-  Lemma fmap_maybe_compose : ∀ (A B C : Type) (f : A → B) (g : B → C),
+  Lemma fmap_maybe_compose : ∀ {A B C} (f : A → B) (g : B → C),
     fmap_maybe (f ∘ g) = fmap_maybe f ∘ fmap_maybe g.
   Proof. simple_solve. Qed.
+  Arguments fmap_maybe_compose [A B C] f g.
 
   Global Instance functor_maybe : Functor (Maybe) := 
   {
     fmap := fmap_maybe;
-    fmap_id := fmap_maybe_id;
+    fmap_id := @fmap_maybe_id;
     fmap_compose := fmap_maybe_compose;
   }.
 End Maybe_Functor.
 Hint Unfold fmap_maybe : soundness.
-Hint Rewrite fmap_maybe_id fmap_maybe_compose : soundness.
+Hint Rewrite @fmap_maybe_id @fmap_maybe_compose : soundness.
 
 Section Maybe_Applicative.
-  Definition app_maybe {A B : Type} 
+  Definition app_maybe {A B} 
     (Mf : Maybe (A -> B)) (Ma : Maybe A) : Maybe B :=
     match Mf, Ma with
     | None, _ => None
     | _, None => None
     | Just f, Just x => Just (f x)
     end.
-  Arguments app_maybe [_ _] _ _.
+  Arguments app_maybe [A B] Mf Ma.
   Hint Unfold app_maybe : soundness.
 
   Lemma app_maybe_id : 
-    ∀ (A : Type) (f : Maybe A), app_maybe (Just id) f = f.
+    ∀ {A} (f : Maybe A), app_maybe (Just id) f = f.
   Proof. simple_solve. Qed.
+  Arguments app_maybe_id [A].
 
   Lemma app_maybe_homomorphism :
-    ∀ (A B : Type) (f : A → B) (x : A), 
+    ∀ {A B} (f : A → B) (x : A), 
     app_maybe (Just f) (Just x) = Just (f x).
   Proof. simple_solve. Qed.
+  Arguments app_maybe_homomorphism [A B] f x.
 
   Lemma app_maybe_interchange :
-    ∀ (A B : Type) (u : Maybe (A → B)) (y : A),
+    ∀ {A B} (u : Maybe (A → B)) (y : A),
     app_maybe u (Just y) = app_maybe (Just (λ f : A → B, f y)) u.
   Proof. simple_solve. Qed.
+  Arguments app_maybe_interchange [A B] u y.
 
   Lemma app_maybe_compose :
-    ∀ (A B C : Type) (u : Maybe (B → C)) (v : Maybe (A → B)) (w : Maybe A),
+    ∀ {A B C} (u : Maybe (B → C)) (v : Maybe (A → B)) (w : Maybe A),
     app_maybe u (app_maybe v w) =
     app_maybe (app_maybe (app_maybe (Just compose) u) v) w.
   Proof. simple_solve. Qed.
+  Arguments app_maybe_compose [A B C] u v w.
 
-  Lemma app_maybe_fmap : ∀ (A B : Type) (f : A → B) (x : Maybe A), 
+  Lemma app_maybe_fmap : ∀ {A B} (f : A → B) (x : Maybe A), 
     fmap f x = app_maybe (Just f) x.
   Proof. simple_solve. Qed.
+  Arguments app_maybe_fmap [A B] f x.
 
   Global Instance applicative_maybe : Applicative Maybe :=
   {
@@ -86,30 +98,51 @@ Section Maybe_Applicative.
   }. 
 End Maybe_Applicative.
 Hint Unfold app_maybe : soundness.
-Hint Rewrite app_maybe_id app_maybe_homomorphism : soundness.
+Hint Rewrite @app_maybe_id @app_maybe_homomorphism : soundness.
 
 Section Maybe_Monad.
-  Definition bind_maybe {A B : Type} 
+  Definition bind_maybe {A B} 
     (m : Maybe A) (k : A -> Maybe B) : Maybe B :=
     match m with
     | None => None
     | Just a => k a
     end.
-  Arguments bind_maybe [_ _].
+  Arguments bind_maybe [A B].
   Hint Unfold bind_maybe : soundness.
 
-  Lemma bind_maybe_id_left : ∀ (A B : Type) (f : A → Maybe B) (a : A), 
+  Lemma bind_maybe_id_left : ∀ {A B} (f : A → Maybe B) (a : A), 
     bind_maybe (Just a) f = f a.
   Proof. simple_solve. Qed.
+  Arguments bind_maybe_id_left [A B] f a.
 
-  Lemma bind_maybe_id_right : ∀ (A : Type) (MA : Maybe A), 
+  Lemma bind_maybe_id_right : ∀ {A} (MA : Maybe A), 
     bind_maybe MA Just = MA.
   Proof. simple_solve. Qed.
+  Arguments bind_maybe_id_right [A].
 
-  Lemma bind_maybe_assoc : ∀ (A B C : Type) (MA : Maybe A) 
+  Lemma bind_maybe_assoc : ∀ {A B C} (MA : Maybe A) 
     (f : A → Maybe B) (g : B → Maybe C),
   bind_maybe (bind_maybe MA f) g = bind_maybe MA (λ a : A, bind_maybe (f a) g).
   Proof. simple_solve. Qed.
+  Arguments bind_maybe_assoc [A B C] MA f g.
+
+  Lemma bind_maybe_app : ∀ {A B} (mf : Maybe (A → B)) (ma : Maybe A),
+    mf <*> ma =
+  bind_maybe mf (λ f : A → B, bind_maybe ma (λ a : A, (f ∘ pure) a)).
+  Proof. simple_solve. Qed.
+  Arguments bind_maybe_app [A B] mf ma.
+
+  Lemma bind_maybe_fmap : ∀ {A B C} (f : A → B) (x : Maybe A) (g : B → Maybe C),
+    bind_maybe (f <$> x) g = bind_maybe x (f ∘ g).
+  Proof. 
+    intros. unfold bind_maybe. unfold compose. destruct x; reflexivity.
+  Qed.
+  Arguments bind_maybe_fmap [A B C] f x g.
+
+  Lemma bind_maybe_pass : ∀ {A B : Type} (ma : Maybe A) (mb : Maybe B),
+    ma >> mb = bind_maybe ma (λ _ : A, mb).
+  Proof. simple_solve. Qed.
+  Arguments bind_maybe_pass [A B] ma mb.
 
   Global Instance monad_maybe : Monad Maybe :=
   {
@@ -117,9 +150,12 @@ Section Maybe_Monad.
     bind_id_left := bind_maybe_id_left;
     bind_id_right := bind_maybe_id_right;
     bind_assoc := bind_maybe_assoc;
-  }. all: solve_monad. Defined.
+    bind_app := bind_maybe_app;
+    bind_fmap := bind_maybe_fmap;
+    bind_pass := bind_maybe_pass;
+  }. 
 End Maybe_Monad.
-Hint Rewrite bind_maybe_id_left bind_maybe_id_right : soundness.
+Hint Rewrite @bind_maybe_id_left @bind_maybe_id_right : soundness.
 
 Inductive AbstractMaybe (A : Type) : Type :=
   | JustA : A -> AbstractMaybe A
@@ -140,22 +176,24 @@ Section AbstractMaybe_Functor.
   Arguments fmap_abstract_maybe [_ _] _ _.
   Hint Unfold fmap_abstract_maybe : soundness.
 
-  Lemma fmap_abstract_maybe_id : ∀ A : Type, fmap_abstract_maybe (@id A) = id.
+  Lemma fmap_abstract_maybe_id : ∀ {A}, fmap_abstract_maybe (@id A) = id.
   Proof. simple_solve. Qed.
+  Arguments fmap_abstract_maybe_id [A].
 
-  Lemma fmap_abstract_maybe_compose : ∀ (A B C : Type) (f : A → B) (g : B → C),
+  Lemma fmap_abstract_maybe_compose : ∀ {A B C : Type} (f : A → B) (g : B → C),
   fmap_abstract_maybe (f ∘ g) = fmap_abstract_maybe f ∘ fmap_abstract_maybe g.
   Proof. simple_solve. Qed.
+  Arguments fmap_abstract_maybe_compose [A B C] f g.
 
   Global Instance functor_abstract_maybe : Functor AbstractMaybe :=
   {
     fmap := fmap_abstract_maybe;
-    fmap_id := fmap_abstract_maybe_id;
+    fmap_id := @fmap_abstract_maybe_id;
     fmap_compose := fmap_abstract_maybe_compose;
   }.
 End AbstractMaybe_Functor.
 Hint Unfold fmap_abstract_maybe : soundness.
-Hint Rewrite fmap_abstract_maybe_id fmap_abstract_maybe_compose : soundness.
+Hint Rewrite @fmap_abstract_maybe_id @fmap_abstract_maybe_compose : soundness.
 
 Section AbstractMaybe_Applicative.
   Definition app_abstract_maybe {A B : Type} (Mf : AbstractMaybe (A -> B))
@@ -171,32 +209,37 @@ Section AbstractMaybe_Applicative.
   Arguments app_abstract_maybe [_ _] _ _.
   Hint Unfold app_abstract_maybe : soundness.
 
-  Lemma app_abstract_maybe_id : ∀ (A : Type) (f : AbstractMaybe A),
+  Lemma app_abstract_maybe_id : ∀ {A} (f : AbstractMaybe A),
     app_abstract_maybe (JustA id) f = f.
   Proof. simple_solve. Qed.
+  Arguments app_abstract_maybe_id [A].
 
-  Lemma app_abstract_maybe_homomorphism : ∀ (A B : Type) (f : A → B) (x : A),
+  Lemma app_abstract_maybe_homomorphism : ∀ {A B} (f : A → B) (x : A),
   app_abstract_maybe (JustA f) (JustA x) = JustA (f x).
   Proof. simple_solve. Qed.
+  Arguments app_abstract_maybe_homomorphism [A B] f x.
 
-  Lemma app_abstract_maybe_interchange : ∀ (A B : Type) 
+  Lemma app_abstract_maybe_interchange : ∀ {A B}
     (u : AbstractMaybe (A → B)) (y : A),
     app_abstract_maybe u (JustA y) =
     app_abstract_maybe (JustA (λ f : A → B, f y)) u.
   Proof. simple_solve. Qed.
+  Arguments app_abstract_maybe_interchange [A B] u y.
 
-  Lemma app_abstract_maybe_compose : ∀ (A B C : Type) 
+  Lemma app_abstract_maybe_compose : ∀ {A B C} 
     (u : AbstractMaybe (B → C)) (v : AbstractMaybe (A → B)) 
     (w : AbstractMaybe A),
     app_abstract_maybe u (app_abstract_maybe v w) =
     app_abstract_maybe
       (app_abstract_maybe (app_abstract_maybe (JustA compose) u) v) w.
   Proof. simple_solve. Qed.
+  Arguments app_abstract_maybe_compose [A B C] u v w.
 
-  Lemma app_abstract_maybe_fmap : ∀ (A B : Type) (f : A → B) 
+  Lemma app_abstract_maybe_fmap : ∀ {A B} (f : A → B) 
     (x : AbstractMaybe A),
   fmap f x = app_abstract_maybe (JustA f) x.
   Proof. simple_solve. Qed.
+  Arguments app_abstract_maybe_fmap [A B] f x.
 
   Global Instance applicative_abstract_maybe : Applicative AbstractMaybe :=
   {
@@ -209,7 +252,7 @@ Section AbstractMaybe_Applicative.
     app_fmap := app_abstract_maybe_fmap;
   }.
 End AbstractMaybe_Applicative.
-Hint Resolve app_abstract_maybe_id app_abstract_maybe_homomorphism : soundness.
+Hint Resolve @app_abstract_maybe_id @app_abstract_maybe_homomorphism : soundness.
 
 Section AbstractMaybe_Monad.
   Definition bind_maybeA {A B : Type}
@@ -226,37 +269,45 @@ Section AbstractMaybe_Monad.
   Arguments bind_maybeA [_ _].
   Hint Unfold bind_maybeA : soundness.
 
-  Lemma bind_maybeA_id_left : ∀ (A B : Type) (f : A → AbstractMaybe B) (a : A),
+  Lemma bind_maybeA_id_left : ∀ {A B} (f : A → AbstractMaybe B) (a : A),
   bind_maybeA (JustA a) f = f a.
   Proof. simple_solve. Qed.
+  Arguments bind_maybeA_id_left [A B] f a.
 
-  Lemma bind_maybeA_id_right :  ∀ (A : Type) (MA : AbstractMaybe A),
+  Lemma bind_maybeA_id_right :  ∀ {A} (MA : AbstractMaybe A),
     bind_maybeA MA JustA = MA.
   Proof. solve_monad. Qed.
+  Arguments bind_maybeA_id_right [A].
 
-  Lemma bind_maybeA_assoc : ∀ (A B C : Type) (MA : AbstractMaybe A) 
+  Lemma bind_maybeA_assoc : ∀ {A B C} (MA : AbstractMaybe A) 
     (f : A → AbstractMaybe B) (g : B → AbstractMaybe C),
     bind_maybeA (bind_maybeA MA f) g =
     bind_maybeA MA (λ a : A, bind_maybeA (f a) g).
   Proof. solve_monad. Qed.
+  Arguments bind_maybeA_assoc [A B C] MA f g.
 
-  Lemma bind_maybeA_fmap : ∀ (A B C : Type) (f : A → B) 
+  Lemma bind_maybeA_fmap : ∀ {A B C} (f : A → B) 
     (x : AbstractMaybe A) (g : B → AbstractMaybe C),
     bind_maybeA (f <$> x) g = bind_maybeA x (f ∘ g).
   Proof.
-    intros. unfold bind_maybeA. destruct x; unfold compose; reflexivity.
+    unfold bind_maybeA; destruct x; unfold compose; reflexivity.
   Qed.
+  Arguments bind_maybeA_fmap [A B C] f x.
 
-  Lemma bind_maybeA_app : ∀ (A B : Type) (mf : AbstractMaybe (A → B)) 
+  Lemma bind_maybeA_app : ∀ {A B} (mf : AbstractMaybe (A → B)) 
     (ma : AbstractMaybe A),
     mf <*> ma =
     bind_maybeA mf (λ f : A → B, bind_maybeA ma (λ a : A, (f ∘ pure) a)).
-  Proof. solve_monad. Qed.
+  Proof. 
+    intros. unfold app. simpl. simple_solve.
+  Qed.
+  Arguments bind_maybeA_app [A B] mf ma.
 
-  Lemma bind_maybeA_pass : ∀ (A B : Type) (ma : AbstractMaybe A) 
+  Lemma bind_maybeA_pass : ∀ {A B} (ma : AbstractMaybe A) 
     (mb : AbstractMaybe B),
     ma >> mb = bind_maybeA ma (λ _ : A, mb).
   Proof. simple_solve. Qed.
+  Arguments bind_maybeA_pass [A B] ma mb.
 
   Global Instance monad_abstract_maybe : Monad AbstractMaybe :=
   {
@@ -269,74 +320,83 @@ Section AbstractMaybe_Monad.
     bind_pass := bind_maybeA_pass;
   }. 
 End AbstractMaybe_Monad.
-Hint Rewrite bind_maybeA_id_left bind_maybeA_id_right : soundness.
+Hint Rewrite @bind_maybeA_id_left @bind_maybeA_id_right : soundness.
 
-Definition MaybeT (M : Type -> Type) (A : Type) : Type := M (Maybe A).
+Definition MaybeT M A: Type := M (Maybe A).
 
 Section MaybeT_Functor.
-  Context {M : Type -> Type} `{Monad M}.
+  Context {M} `{Monad M}.
 
-  Definition fmap_maybeT {A B : Type} (f : A -> B)
+  Definition fmap_maybeT {A B} (f : A -> B)
     (m : MaybeT M A) : MaybeT M B :=  fmap (fmap (F:=Maybe) f) m. 
   Arguments fmap_maybeT [_ _] _ _.
   Hint Unfold fmap_maybeT : soundness.
 
-  Lemma fmap_maybeT_id : ∀ A : Type, fmap_maybeT (@id A) = id.
+  Lemma fmap_maybeT_id : ∀ {A}, fmap_maybeT (@id A) = id.
   Proof. simple_solve. Qed.
+  Arguments fmap_maybeT_id [A].
 
-  Lemma fmap_maybeT_compose : ∀ (A B C : Type) (f : A → B) (g : B → C),
+  Lemma fmap_maybeT_compose : ∀ {A B C} (f : A → B) (g : B → C),
   fmap_maybeT (f ∘ g) = fmap_maybeT f ∘ fmap_maybeT g.
-  Proof. simple_solve. Qed.
+  Proof. 
+    intros. unfold fmap_maybeT. ext.
+    repeat rewrite fmap_compose. 
+    reflexivity.
+  Qed.
+  Arguments fmap_maybeT_compose [A B C] f g.
 
   Global Instance functor_maybeT : Functor (MaybeT M) :=
   {
     fmap := fmap_maybeT;
-    fmap_id := fmap_maybeT_id;
+    fmap_id := @fmap_maybeT_id;
     fmap_compose := fmap_maybeT_compose;
   }.
 End MaybeT_Functor.
 Hint Unfold fmap_maybeT : soundness.
-Hint Rewrite fmap_maybeT_id fmap_maybeT_compose : soundness.
+Hint Rewrite @fmap_maybeT_id @fmap_maybeT_compose : soundness.
 
 Section MaybeT_Applicative.
-  Context {M : Type -> Type} `{inst : Monad M}.
+  Context {M} `{inst : Monad M}.
 
-  Definition pure_maybeT {A : Type} (x : A) : MaybeT M A :=
+  Definition pure_maybeT {A} (x : A) : MaybeT M A :=
     pure (Just x).
   Arguments pure_maybeT [_] _.
   Hint Unfold pure_maybeT : soundness.
 
-  Definition app_maybeT {A B : Type} (Mmf : MaybeT M (A -> B))
+  Definition app_maybeT {A B} (Mmf : MaybeT M (A -> B))
     (Mma : MaybeT M A) : MaybeT M B := 
-    @bindM M _ _ inst _ _ Mmf (λ mf : Maybe (A → B), 
+    @bindM M _ _ _ Mmf (λ mf : Maybe (A → B), 
       match mf with
       | Just f =>
-          @bindM M _ _ inst _ _ Mma (λ ma : Maybe A, 
+          @bindM M _ _ _ Mma (λ ma : Maybe A, 
             match ma with
             | Just a => pure (Just (f a))
             | None => pure None
             end)
       | None => pure None
       end).
-  Arguments app_maybeT [_ _] _ _.
+  Arguments app_maybeT [A B] Mmf Mma.
   Hint Unfold app_maybeT : soundness.
 
-  Lemma app_maybeT_id : ∀ (A : Type) (f : M (Maybe A)),
+  Lemma app_maybeT_id : ∀ {A} (f : M (Maybe A)),
     app_maybeT (pure_maybeT id) f = f.
   Proof. 
     solve_monad. rewrite <- (bind_id_right (M:=M)). 
     f_equal; ext. destruct x; reflexivity.
   Qed.
+  Arguments app_maybeT_id [A] f.
 
-  Lemma app_maybeT_homomorphism : ∀ (A B : Type) (f : A → B) (x : A),
+  Lemma app_maybeT_homomorphism : ∀ {A B} (f : A → B) (x : A),
   app_maybeT (pure_maybeT f) (pure_maybeT x) = pure_maybeT (f x).
   Proof. solve_monad. Qed.
+  Arguments app_maybeT_homomorphism [A B] f x.
 
-  Lemma app_maybeT_interchange : ∀ (A B : Type) (u : MaybeT M (A → B)) (y : A),
+  Lemma app_maybeT_interchange : ∀ {A B} (u : MaybeT M (A → B)) (y : A),
   app_maybeT u (pure_maybeT y) = app_maybeT (pure_maybeT (λ f : A → B, f y)) u.
   Proof. solve_monad. Qed.
+  Arguments app_maybeT_interchange [A B] u y.
 
-  Lemma app_maybeT_compose : ∀ (A B C : Type) (u : MaybeT M (B → C)) 
+  Lemma app_maybeT_compose : ∀ {A B C} (u : MaybeT M (B → C)) 
     (v : MaybeT M (A → B))  (w : MaybeT M A),
     app_maybeT u (app_maybeT v w) =
     app_maybeT (app_maybeT (app_maybeT (pure_maybeT compose) u) v) w.
@@ -348,13 +408,14 @@ Section MaybeT_Applicative.
     reflexivity. rewrite bind_id_left. reflexivity. repeat rewrite bind_id_left.
     reflexivity. repeat rewrite bind_id_left. reflexivity.
   Qed.
+  Arguments app_maybeT_compose [A B C] u v w.
 
-  Lemma fmap_app_maybeT : ∀ (A B : Type) (f : A → B) (x : MaybeT M A),
+  Lemma fmap_app_maybeT : ∀ {A B} (f : A → B) (x : MaybeT M A),
   fmap_maybeT f x = app_maybeT (pure_maybeT f) x.
   Proof. 
-    solve_monad. rewrite fmap_bind_pure. f_equal; ext. 
-    unfold compose. destruct x0; reflexivity.
+    solve_monad.
   Qed.
+  Arguments fmap_app_maybeT [A B] f x.
 
   Global Instance applicative_maybeT : Applicative (MaybeT M) :=
   {
@@ -368,58 +429,66 @@ Section MaybeT_Applicative.
   }. 
 End MaybeT_Applicative.
 Hint Unfold pure_maybeT app_maybeT : soundness.
-Hint Rewrite app_maybeT_id app_maybeT_homomorphism : soundness.
+Hint Rewrite @app_maybeT_id @app_maybeT_homomorphism : soundness.
 
 Section MaybeT_Monad.
-  Context {M : Type -> Type} `{inst : Monad M}.
+  Context {M} `{inst : Monad M}.
 
-  Definition bind_maybeT {A B : Type} (x : MaybeT M A)
+  Definition bind_maybeT {A B} (x : MaybeT M A)
     (f : A -> MaybeT M B) : MaybeT M B :=
-    @bindM M _ _ inst (Maybe A) (Maybe B) x (fun v =>
+    @bindM M _ (Maybe A) (Maybe B) x (fun v =>
       match v with
       | None => pure None
       | Just a => f a
       end
     ).
-  Arguments bind_maybeT [_ _] _ _.
+  Arguments bind_maybeT [A B] x f.
   Hint Unfold bind_maybeT : soundness.
 
-  Lemma bind_maybeT_id_left : ∀ (A B : Type) (f : A → MaybeT M B) (a : A), 
+  Lemma bind_maybeT_id_left : ∀ {A B} (f : A → MaybeT M B) (a : A), 
     bind_maybeT (pure a) f = f a.
-  Proof. solve_monad. Qed.
+  Proof. 
+    intros. unfold bind_maybeT. unfold pure. simpl. unfold pure_maybeT.
+    rewrite bind_id_left. reflexivity.
+  Qed.
+  Arguments bind_maybeT_id_left [A B] f a.
 
-  Lemma bind_maybeT_id_right : ∀ (A : Type) (MA : MaybeT M A),
+  Lemma bind_maybeT_id_right : ∀ {A} (MA : MaybeT M A),
     bind_maybeT MA pure = MA.
   Proof. 
     solve_monad. rewrite <- (bind_id_right (M:=M)). f_equal. 
     ext; destruct x; reflexivity.
   Qed.
+  Arguments bind_maybeT_id_right [A] MA.
 
-  Lemma bind_maybeT_assoc : ∀ (A B C : Type) (MA : MaybeT M A) 
+  Lemma bind_maybeT_assoc : ∀ {A B C} (MA : MaybeT M A) 
     (f : A → MaybeT M B) (g : B → MaybeT M C),
     bind_maybeT (bind_maybeT MA f) g =
     bind_maybeT MA (λ a : A, bind_maybeT (f a) g).
   Proof. solve_monad. Qed.
+  Arguments bind_maybeT_assoc [A B C] MA f g.
 
-  Lemma bind_maybeT_app : ∀ (A B : Type) (mf : MaybeT M (A → B)) 
+  Lemma bind_maybeT_app : ∀ {A B} (mf : MaybeT M (A → B)) 
     (ma : MaybeT M A),
     mf <*> ma = 
     bind_maybeT mf (λ f : A → B, bind_maybeT ma (λ a : A, (f ∘ pure) a)).
-  Proof. 
-    intros. simpl. unfold app_maybeT, pure_maybeT, bind_maybeT.
-    f_equal; ext.
-  Qed.
+  Proof. simple_solve. Qed.
+  Arguments bind_maybeT_app [A B] mf ma.
 
-  Lemma bind_maybeT_fmap : ∀ (A B C : Type) (f : A → B) 
+  Lemma bind_maybeT_fmap : ∀ {A B C} (f : A → B) 
     (x : MaybeT M A) (g : B → MaybeT M C),
     bind_maybeT (fmap f x) g = bind_maybeT x (f ∘ g).
-  Proof. solve_monad. Qed.
-
-  Lemma bind_maybeT_pass : ∀ (A B : Type) (ma : MaybeT M A) (mb : MaybeT M B),
-    ma >> mb = bind_maybeT ma (λ _ : A, mb).
-  Proof.
-    solve_monad.
+  Proof. 
+    intros. unfold bind_maybeT. unfold fmap; simpl. unfold fmap_maybeT.
+    rewrite bind_fmap. f_equal. ext. unfold compose. 
+    destruct x0; reflexivity.
   Qed.
+  Arguments bind_maybeT_fmap [A B C] f x g.
+
+  Lemma bind_maybeT_pass : ∀ {A B} (ma : MaybeT M A) (mb : MaybeT M B),
+    ma >> mb = bind_maybeT ma (λ _ : A, mb).
+  Proof. solve_monad. Qed.
+  Arguments bind_maybeT_pass [A B] ma mb.
 
   Global Instance monad_maybeT : Monad (MaybeT M) :=
   {
@@ -433,14 +502,14 @@ Section MaybeT_Monad.
   }. 
 End MaybeT_Monad.
 Hint Unfold bind_maybeT : soundness.
-Hint Rewrite bind_maybeT_id_left 
-             bind_maybeT_id_right 
-             bind_maybeT_app bind_maybeT_fmap : soundness.
+Hint Rewrite @bind_maybeT_id_left 
+             @bind_maybeT_id_right 
+             @bind_maybeT_app @bind_maybeT_fmap : soundness.
 
 Section MaybeT_MonadT.
-  Context {M : Type -> Type} `{Monad M}.
+  Context {M} `{Monad M}.
   
-  Definition lift_maybeT {A : Type} (Ma : M A) : M (Maybe A) :=
+  Definition lift_maybeT {A} (Ma : M A) : M (Maybe A) :=
     fmap Just Ma.
   Arguments lift_maybeT [_] _.
   Hint Unfold lift_maybeT : soundness.
@@ -452,15 +521,15 @@ Section MaybeT_MonadT.
   }. all: solve_monad. Defined.
 End MaybeT_MonadT.
 
-Definition MaybeAT (M : Type -> Type) (A : Type) : Type := M (AbstractMaybe A).
+Definition MaybeAT M A : Type := M (AbstractMaybe A).
 
 Section MaybeAT_Functor.
-  Context {M : Type -> Type} `{inst : Functor M}.
+  Context {M} `{inst : Functor M}.
 
-  Definition fmap_maybeAT {A B : Type} 
+  Definition fmap_maybeAT {A B} 
     (f : A -> B) (Ma : MaybeAT M A) : MaybeAT M B :=
     fmap (fmap_abstract_maybe f) Ma.
-  Arguments fmap_maybeAT [_ _] _ _.
+  Arguments fmap_maybeAT [A B] f Ma.
   Hint Unfold fmap_maybeAT : soundness.
 
   Global Instance functor_maybeAT : Functor (MaybeAT M) :=
@@ -477,76 +546,79 @@ End MaybeAT_Functor.
 Hint Unfold fmap_maybeAT : soundness.
 
 Section MaybeAT_Applicative.
-  Context {M : Type -> Type} `{inst : Monad M}.
+  Context {M} `{inst : Monad M}.
 
-  Definition pure_maybeAT {A : Type} (x : A) : MaybeAT M A :=
+  Definition pure_maybeAT {A} (x : A) : MaybeAT M A :=
     pure (JustA x).
-  Arguments pure_maybeAT [_] _.
+  Arguments pure_maybeAT [A] x.
   Hint Unfold pure_maybeAT : soundness.
 
-  Definition app_maybeT' {A B : Type} (Mmf : MaybeT M (A -> B))
-    (Mma : MaybeT M A) : MaybeT M B := 
-    @bindM M _ _ inst _ _ Mmf (λ mf : Maybe (A → B), 
-      match mf with
-      | Just f =>
-          @bindM M _ _ inst _ _ Mma (λ ma : Maybe A, 
-            match ma with
-            | Just a => pure (Just (f a))
-            | None => pure None
-            end)
-      | None => pure None
-      end).
-  Definition app_maybeAT {A B : Type} (Mmf : MaybeAT M (A -> B))
+  Definition app_maybeAT {A B} (Mmf : MaybeAT M (A -> B))
     (Mma : MaybeAT M A) : MaybeAT M B :=
-    @bindM M _ _ inst _ _ Mmf 
+    @bindM M _ _ _ Mmf 
       (λ mf : AbstractMaybe (A -> B),
       match mf with 
-      | JustA f => @bindM M _ _ inst _ _ Mma 
+      | JustA f => @bindM M _ _ _ Mma 
           (λ ma : AbstractMaybe A,
           match ma with
           | JustOrNoneA a => pure (F:=M) (JustOrNoneA (f a))
           | JustA a => pure (F:=M) (JustA (f a))
           | NoneA => pure (F:=M) NoneA
           end)
-      | JustOrNoneA f => @bindM M _ _ inst _ _ Mma (λ ma : AbstractMaybe A,
+      | JustOrNoneA f => @bindM M _ _ _ Mma (λ ma : AbstractMaybe A,
           match ma with
           | JustA a | JustOrNoneA a => pure (F:=M) (JustOrNoneA (f a))
           | NoneA => pure (F:=M) NoneA
           end)
       | NoneA => pure (F:=M) NoneA
       end).
-  Arguments app_maybeAT [_ _] _ _.
+  Arguments app_maybeAT [A B] Mmf Mma.
   Hint Unfold app_maybeAT : soundness.
 
-  Lemma app_maybeAT_id : ∀ (A : Type) (f : MaybeAT M A), 
+  Lemma app_maybeAT_id : ∀ {A} (f : MaybeAT M A), 
     app_maybeAT (pure_maybeAT id) f = f.
   Proof. 
     solve_monad. rewrite <- (bind_id_right (M:=M)). f_equal; ext.
     destruct x; reflexivity.
   Qed.
+  Arguments app_maybeAT_id [A] f.
 
-  Lemma app_maybeAT_homomorphism : ∀ (A B : Type) (f : A → B) (x : A),
+  Lemma app_maybeAT_homomorphism : ∀ {A B} (f : A → B) (x : A),
     app_maybeAT (pure_maybeAT f) (pure_maybeAT x) = pure_maybeAT (f x).
   Proof. solve_monad. Qed.
+  Arguments app_maybeAT_homomorphism [A B] f x.
 
-  Lemma app_maybeAT_interchange : ∀ (A B : Type) (u : MaybeAT M (A → B)) (y : A),
+  Lemma app_maybeAT_interchange : ∀ {A B} (u : MaybeAT M (A → B)) (y : A),
     app_maybeAT u (pure_maybeAT y) = 
     app_maybeAT (pure_maybeAT (λ f : A → B, f y)) u.
   Proof. solve_monad. Qed.
+  Arguments app_maybeAT_interchange [A B] u y.
 
-  Lemma app_maybeAT_compose : ∀ (A B C : Type) 
+  Lemma app_maybeAT_compose : ∀ {A B C}
     (u : MaybeAT M (B → C)) (v : MaybeAT M (A → B)) (w : MaybeAT M A),
     app_maybeAT u (app_maybeAT v w) =
     app_maybeAT (app_maybeAT (app_maybeAT (pure_maybeAT compose) u) v) w.
-  Proof. solve_monad. Qed.
+  Proof. 
+    intros; unfold app_maybeAT, pure_maybeAT; rewrite bind_id_left;
+    repeat rewrite bind_assoc; f_equal; ext; destruct x; 
+    repeat rewrite bind_id_left; try reflexivity;
+    repeat rewrite bind_assoc; f_equal; ext; destruct x;
+    repeat rewrite bind_id_left; try reflexivity;
+    repeat rewrite bind_assoc; f_equal; ext; destruct x;
+    repeat rewrite bind_id_left; reflexivity.
+  Qed.
   Hint Unfold fmap_maybeAT : soundness.
+  Arguments app_maybeAT_compose [A B C] u v w.
 
-  Lemma app_maybeAT_fmap : ∀ (A B : Type) (f : A → B) (x : MaybeAT M A),
+  Lemma app_maybeAT_fmap : ∀ {A B} (f : A → B) (x : MaybeAT M A),
     f <$> x = app_maybeAT (pure_maybeAT f) x.
   Proof.
-    solve_monad. unfold fmap_abstract_maybe. rewrite fmap_bind_pure.
+    intros. unfold app_maybeAT, pure_maybeAT. rewrite bind_id_left.
+    unfold fmap; simpl. unfold fmap_maybeAT.
+    unfold fmap_abstract_maybe. rewrite fmap_bind_pure.
     f_equal; ext. unfold compose. destruct x0; reflexivity.
   Qed.
+  Arguments app_maybeAT_fmap [A B] f x.
 
   Global Instance applicative_maybeAT : Applicative (MaybeAT M) :=
   {
@@ -562,58 +634,70 @@ End MaybeAT_Applicative.
 Hint Unfold pure_maybeAT app_maybeAT : soundness.
 
 Section MaybeAT_Monad.
-  Context {M : Type -> Type} `{inst : Monad M}.
+  Context {M} `{inst : Monad M}.
 
   Definition bind_maybeAT {A B} 
     (Mma : M (AbstractMaybe A))
     (f : A -> M (AbstractMaybe B)) : M (AbstractMaybe B) :=
-  @bindM M _ _ inst (AbstractMaybe A) (AbstractMaybe B) Mma (fun ma =>
+  @bindM M _ (AbstractMaybe A) (AbstractMaybe B) Mma (fun ma =>
     match ma with
     | NoneA => pure NoneA
     | JustA a => f a
     | JustOrNoneA a => 
-        @bindM M _ _ inst (AbstractMaybe B) (AbstractMaybe B) (f a) (fun mfa =>
+        @bindM M _ (AbstractMaybe B) (AbstractMaybe B) (f a) (fun mfa =>
                        match mfa with
                        | NoneA => pure NoneA
                        | JustA b => pure (JustOrNoneA b)
                        | JustOrNoneA b => pure (JustOrNoneA b)
                        end)
     end).
-  Arguments bind_maybeAT [_ _].
+  Arguments bind_maybeAT [A B] Mma f.
   Hint Unfold bind_maybeAT : soundness.
 
-  Lemma bind_maybeAT_id_left : ∀ (A B : Type) (f : A → MaybeAT M B) (a : A), 
+  Lemma bind_maybeAT_id_left : ∀ {A B} (f : A → MaybeAT M B) (a : A), 
     bind_maybeAT (pure a) f = f a.
-  Proof. solve_monad. Qed.
+  Proof. 
+    unfold pure; simpl. solve_monad. 
+  Qed.
+  Arguments bind_maybeAT_id_left [A B] f a.
 
-  Lemma bind_maybeAT_id_right : ∀ (A : Type) (MA : MaybeAT M A), 
+  Lemma bind_maybeAT_id_right : ∀ {A} (MA : MaybeAT M A), 
     bind_maybeAT MA pure = MA.
-  Proof. solve_monad. Qed.
+  Proof. 
+    unfold pure. solve_monad. 
+  Qed.
+  Arguments bind_maybeAT_id_right [A] MA.
 
-  Lemma bind_maybeAT_assoc : ∀ (A B C : Type) (MA : MaybeAT M A) 
+  Lemma bind_maybeAT_assoc : ∀ {A B C} (MA : MaybeAT M A) 
     (f : A → MaybeAT M B) (g : B → MaybeAT M C),
     bind_maybeAT (bind_maybeAT MA f) g =
     bind_maybeAT MA (λ a : A, bind_maybeAT (f a) g).
   Proof. solve_monad. Qed.
+  Arguments bind_maybeAT_assoc [A B C] MA f g.
 
-  Lemma bind_maybeAT_app : ∀ (A B : Type) (mf : MaybeAT M (A → B)) 
+  Lemma bind_maybeAT_app : ∀ {A B} (mf : MaybeAT M (A → B)) 
     (ma : MaybeAT M A), mf <*> ma =
     bind_maybeAT mf (λ f : A → B, bind_maybeAT ma (λ a : A, (f ∘ pure) a)).
   Proof.
+    unfold pure, app.
     solve_monad.
   Qed.
+  Arguments bind_maybeAT_app [A B] mf ma.
 
-  Lemma bind_maybeAT_fmap : ∀ (A B C : Type) (f : A → B) (x : MaybeAT M A) 
+  Lemma bind_maybeAT_fmap : ∀ {A B C} (f : A → B) (x : MaybeAT M A) 
     (g : B → MaybeAT M C), bind_maybeAT (f <$> x) g = bind_maybeAT x (f ∘ g).
   Proof.
+    unfold fmap.
     solve_monad.
   Qed.
+  Arguments bind_maybeAT_fmap [A B C] f x g.
 
-  Lemma bind_maybeAT_pass : ∀ (A B : Type) (ma : MaybeAT M A) 
+  Lemma bind_maybeAT_pass : ∀ {A B} (ma : MaybeAT M A) 
     (mb : MaybeAT M B), ma >> mb = bind_maybeAT ma (λ _ : A, mb).
   Proof.
     solve_monad.
   Qed.
+  Arguments bind_maybeAT_pass [A B] ma mb.
 
   Global Instance monad_maybeAT 
   : Monad (MaybeAT M) :=
@@ -630,24 +714,26 @@ End MaybeAT_Monad.
 Hint Unfold bind_maybeAT : soundness.
 
 Section MaybeAT_MonadT.
-  Context {M : Type -> Type} `{Monad M}.
+  Context {M} `{Monad M}.
 
-  Definition lift_maybeAT {A : Type} (Ma : M A) : MaybeAT M A :=
+  Definition lift_maybeAT {A} (Ma : M A) : MaybeAT M A :=
     fmap JustA Ma.
-  Arguments lift_maybeAT [_].
+  Arguments lift_maybeAT [A].
   Hint Unfold lift_maybeAT : soundness.
 
-  Definition lift_maybeAT_pure : ∀ (A : Type) (x : A),
+  Definition lift_maybeAT_pure : ∀ {A} (x : A),
     lift_maybeAT (pure x) = pure x.
   Proof.
     solve_monad.
   Qed.
+  Arguments lift_maybeAT_pure [A] x.
 
-  Definition lift_maybeAT_bind : ∀ (A B : Type) (x : M A) (f : A → M B),
+  Definition lift_maybeAT_bind : ∀ {A B} (x : M A) (f : A → M B),
     lift_maybeAT (x >>= f) = lift_maybeAT x >>= (f ∘ lift_maybeAT (A:=B)).
   Proof. 
     solve_monad.
   Qed.
+  Arguments lift_maybeAT_bind [A B] x f.
 
   Global Instance monadT_maybeAT : MonadT MaybeAT :=
   {
@@ -661,14 +747,13 @@ End MaybeAT_MonadT.
 Definition State (S A : Type) := S -> (A * S).
 
 Section State_Functor.
-  
-  Definition fmap_state {S A B : Type} 
+  Definition fmap_state {S A B} 
     (f : A -> B) (Fa : State S A) : State S B :=
   fun st => let (x, s) := Fa st in (f x, s).
-  Arguments fmap_state [_ _ _] _ _.
+  Arguments fmap_state [S A B] f Fa.
   Hint Unfold fmap_state : soundness.
 
-  Global Instance functor_state (S : Type) : Functor (State S) :=
+  Global Instance functor_state {S} : Functor (State S) :=
   {
     fmap := @fmap_state S;
   }. all: solve_monad. Defined.
@@ -677,51 +762,54 @@ End State_Functor.
 Hint Unfold fmap_state : soundness.
 
 Section State_Applicative.
-  Definition pure_state {S A : Type} (a : A) : State S A :=
+  Definition pure_state {S A} (a : A) : State S A :=
     fun st => (a, st).
+  Arguments pure_state [S A] a.
 
-  Definition app_state {S A B : Type} 
+  Definition app_state {S A B} 
     (Mf : State S (A -> B)) (Ma : State S A) : State S B :=
     fun st => let (f, st') := Mf st in 
               let (a, st'') := Ma st' in (f a, st'').
+  Arguments app_state [S A B] Mf Ma.
   Hint Unfold pure_state app_state : soundness.
 
-  Global Instance applicative_state (S : Type) : Applicative (State S) :=
+  Global Instance applicative_state S : Applicative (State S) :=
   {
     pure := @pure_state S;
     app := @app_state S;
-  }. all: solve_monad. Defined.
+  }. all: unfold fmap; solve_monad. Defined.
 End State_Applicative.
 Hint Unfold app_state : soundness.
 
 Section State_Monad.
-  Definition bind_state {S A B : Type} 
+  Definition bind_state {S A B} 
     (p : State S A) (k : A -> State S B) : State S B :=
     fun st => match (p st) with
               | (x, st') => k x st'
               end.
+  Arguments bind_state [S A B] p k.
   Hint Unfold bind_state : soundness.
 
   Global Instance monad_state (S : Type) :  Monad (State S) :=
   {
     bindM := @bind_state S;
-  }. all: solve_monad. Defined.
+  }. all: unfold fmap, app; solve_monad. Defined.
 End State_Monad.
 Hint Unfold bind_state : soundness.
 
-Definition StateT (S : Type) (M : Type -> Type) (A : Type) : Type :=
-  S -> M (A*S)%type.
+Definition StateT S M A : Type := S → M (A*S)%type.
 
 Section Functor_StateT.
-  Context {M : Type -> Type} `{Monad M}.
+  Context {M} `{Monad M}.
 
-  Definition fmap_stateT {S A B : Type} (f : A -> B) (m : StateT S M A)
+  Definition fmap_stateT {S A B} (f : A -> B) (m : StateT S M A)
     : StateT S M B :=
     fun s : S => bindM (m s) 
       (fun x => let (a, s') := x : (A*S)%type in pure (f a, s')).
+  Arguments fmap_stateT [S A B] f m.
   Hint Unfold fmap_stateT : soundness.
 
-  Global Instance functor_stateT (S : Type) : Functor (StateT S M) :=
+  Global Instance functor_stateT S : Functor (StateT S M) :=
   {
     fmap := @fmap_stateT S;
   }. all: solve_monad. Defined.
@@ -729,21 +817,23 @@ End Functor_StateT.
 Hint Unfold fmap_stateT : soundness.
 
 Section Applicative_StateT.
-  Context {M : Type -> Type} `{Monad M}.
+  Context {M} `{Monad M}.
 
-  Definition pure_stateT {S A : Type} (x : A) : StateT S M A :=
+  Definition pure_stateT {S A} (x : A) : StateT S M A :=
     fun s => pure (x, s).
+  Arguments pure_stateT [S A] x.
 
   Definition app_stateT
-    {S A B : Type}
+    {S A B}
     (sf : StateT S M (A -> B)) (sa : StateT S M A) : StateT S M B :=
     fun st : S =>
     bindM (sf st) (fun '(f, stf) =>
       bindM (sa stf) (fun '(a, sta) =>
         pure (f a, sta))).
+  Arguments app_stateT [S A B] sf sa.
   Hint Unfold pure_stateT app_stateT : soundness.
 
-  Global Instance applicative_stateT (S : Type) : Applicative (StateT S M) :=
+  Global Instance applicative_stateT S : Applicative (StateT S M) :=
   {
     pure := @pure_stateT S;
     app := @app_stateT S;
@@ -752,29 +842,31 @@ End Applicative_StateT.
 Hint Unfold pure_stateT app_stateT : soundness.
 
 Section Monad_StateT.
-  Context {M : Type -> Type} `{Monad M}.
+  Context {M} `{Monad M}.
 
-  Definition bind_stateT {S A B : Type} 
+  Definition bind_stateT {S A B} 
     (MA : StateT S M A) (f : A -> StateT S M B) : StateT S M B :=
     fun st => bindM (MA st) 
       (fun p : (A*S)%type => let (a,st') := p in f a st').
+  Arguments bind_stateT [S A B] MA f.
   Hint Unfold bind_stateT : soundness.
 
-  Global Instance monad_stateT (S : Type) : Monad (StateT S M) :=
+  Global Instance monad_stateT S : Monad (StateT S M) :=
   {
     bindM := @bind_stateT S;
-  }. all: solve_monad. Defined.
+  }. all: unfold pure, fmap; solve_monad. Defined.
 End Monad_StateT.
 Hint Unfold bind_stateT : soundness.
 
 Section MonadT_StateT.
-  Context {M : Type -> Type} `{Monad M}.
+  Context {M} `{Monad M}.
 
-  Definition lift_stateT {S A : Type} (MA : M A) : StateT S M A :=
+  Definition lift_stateT {S A} (MA : M A) : StateT S M A :=
     fun st => bindM MA (fun a => pure (a, st)).
+  Arguments lift_stateT [S A] MA.
   Hint Unfold lift_stateT : soundness.
 
-  Global Instance monadT_stateT (S : Type) : MonadT (StateT S) :=
+  Global Instance monadT_stateT S : MonadT (StateT S) :=
   {
     liftT := @lift_stateT S;
   }. all: solve_monad. Defined.
